\documentclass {article}

\newcommand\reals{\mathbf{R}}
\newcommand\bernstein[2]{b_{#1, #2}}
\begin{document}

\section{Polynom}

$$
P (t) = \sum_{i=0}^n P_i \times b_i(\frac{t - t_0}{T})
$$

where $t \in \left[ t_0, t_0 + T \right]$, $(b_i)$ is a basis of the polynoms
of degree less or equal to $n$ and $(P_i)$ is a set of points.

\paragraph{Derivative}

$$
P^{(k)} (t) = \sum_{i=0}^n \frac{P_i}{T^k} \times b_i^{(k)}(\frac{t - t_0}{T})
$$

\paragraph{Integral of derivatives}
\begin{eqnarray*}
\int_{t_{min}}^{t_{min} + T} {P^{(k)} (t)}^T . P^{(k)} (t) dt
&=& \sum_{i,j} \frac{P_i^T P_j}{T^{2k}} \int_{t_{min}}^{t_{min} + T} b_i^{(k)}(\frac{t - t_0}{T}) b_j^{(k)}(\frac{t - t_0}{T}) dt \\
&=& \sum_{i,j} \frac{P_i^T P_j}{T^{2k}} T \int_0^1 b_i^{(k)}(u) b_j^{(k)}(u) du \\
&=& T^{1-2k} \sum_{i,j} P_i^T P_j \int_0^1 b_i^{(k)}(u) b_j^{(k)}(u) du \\
\end{eqnarray*}

\section{Definiton of some basis}

We consider $u \in \left[ 0,1 \right]$.

\subsection {Canonical polynom basis}

$$
b_i(u) = u^i
$$

Its $k$-th derivative is, for $k \le i$:
$$
b_i^{(k)} (u) = \frac{i!}{(i-k)!} u^{i-k}
$$

Finally,
\begin{eqnarray*}
\int_0^1 b_i^{(k)} (u) b_j^{(k)} (u) du
&=& \frac{i!}{(i-k)!} \frac{j!}{(j-k)!} \int_0^1 u^{i+j-2k} du \\
&=& \frac{i!}{(i-k)!} \frac{j!}{(j-k)!} \frac{1}{i+j-2k+1}
\end{eqnarray*}

\subsection {Bernstein polynoms}
The $i$-th Bernstein polynom of degree $n$ is:
$$
\bernstein{i}{n} (u) = { n \choose i } u^i (1-u)^{n-i}
$$

Its $k$-th derivative is, for $k \le n$:
\begin{eqnarray*}
\bernstein{i}{n}^{(k)} (u) &=& n! \sum_{p = \max(0, k+i-n)}^{\min(k,i)} { k \choose p } (-1)^{k-p} \frac{u^{i-p} (1-u)^{n-k-(i-p)}}{(i-p)!(n-k-(i-p))!} \\
&=& \frac{n!}{(n-k)!} \sum_{p = \max(0, k+i-n)}^{\min(k,i)} { k \choose p } (-1)^{k-p} \bernstein{i-p}{n-k}(u)
\end{eqnarray*}

\paragraph{Integral of product of derivatives}
We seek to compute
\begin{eqnarray*}
  \alpha_{i,j,n}^{(k)} &:=& \int_0^1 \bernstein{i}{n}^{(k)}(u) \bernstein{j}{n}^{(k)} (u) dt \\
& =& \left(\frac{n!}{(n-k)!}\right)^2 \sum_{p \in I(i,k,n), q \in I(j,k,n)} { k \choose p } { k \choose q } (-1)^{2k - (p+q)} \alpha_{i-p,j-q,n-k}^{(0)} \\
\end{eqnarray*}

with $I(i,k,n) = [ \max(0, k+i-n), \min(k,i) ]$

% with:
% $$
% \beta_{i,j}^{n,k} = \int_0^1 \bernstein{i-p}{n-k}(u) \bernstein{j-q}{n-k} (u) dt \\
% $$

\paragraph{Calculation of $\alpha_{i,j,n}^{(0)}$}
\begin{eqnarray*}
  \alpha_{i,j,n}^{(0)}
  &=& { n \choose i } { n \choose j } { 2n \choose i+j }^{-1} \int_0^1 \bernstein{i+j}{2n}(u) dt \\
  &=& { n \choose i } { n \choose j } { 2n \choose i+j }^{-1} \frac{1}{2n + 1}
\end{eqnarray*}

% Thus:
% \begin{eqnarray*}
  % \alpha_{i,j,n}^{(k)}
  % & =& \left(\frac{n!}{(n-k)!}\right)^2 \sum_{p \in I(i,k,n), q \in I(j,k,n)} (-1)^{2k - (p+q)}
  % { k \choose p } { k \choose q } { n-k \choose i-p } { n-k \choose j-q } { 2(n-k) \choose i-p+j-q }^{-1} \frac{1}{2(n-k) + 1}
  % \alpha_{i-p,j-q,n-k}^{(0)} \\
% \end{eqnarray*}

\paragraph{Maximum on an interval}
Let $I = \left[ t_0, t_1 \right] \subset \left[ 0,1 \right]$.

We seek $ M_{i,n} (I) = \max_{u \in I} |\bernstein{i}{n} (u)| $.
Clearly, we have
$$ M_{0, n} (I) = \bernstein{0}{n} (t_0) $$
and
$$ M_{n, n} (I) = \bernstein{n}{n} (t_1) $$

As $\bernstein{i}{n}' (u) = { n \choose i } ( i - u n ) u^{i-1} (1-u)^{n-i-1}$,
we have, $\forall i \in \left[ 1, n-1 \right]$, $ M_{i,n} (I) = \bernstein{i}{n} (t_M(I)) $
where
\begin{equation}
  t_M (I) = \left\lbrace
  \begin{array}{cl}
    t_0 & \textbf{ if } \frac{i}{n} > t_0 \\
    t_1 & \textbf{ if } t_1 < \frac{i}{n} \\
    \frac{i}{n} & \textbf{otherwise}
  \end{array}
  \right.
\end{equation}
The above formula is also true for $i = 0$ and $i=n$.

We seek $ M_{i,n}' (I) = \max_{u \in I} |\bernstein{i}{n}' (u)| $.

$$
\bernstein{i}{n}'' (u) = { n \choose i } \left[ (n-1)^2 u^2 - (2 i - 1) (n - 1) u + i (i-1) \right] u^{i-2} (1-u)^{n-i-2}
$$

Let $ \alpha(u) = (n-1)^2 u^2 - (n - 1)(2 i - 1) u + i (i-1) $.
As $\Delta = (n-1)^2 ( (2i-1)^2 - 4 i (i - 1)) = (n-1)^2$,
the roots of $\alpha$ are $ u_- = \frac{i-1}{n-1} $ and $ u_+ = \frac{i}{n-1}$.
As $(n-1)^2 > 0$, $\bernstein{i}{n}'$ increases on $\left[ 0, u_- \right]$ and on $\left[ u_+, 1\right]$
and decreases on $\left[ u_-, u_+ \right]$.

$$
\bernstein{i}{n}' (u_-) = { n \choose i } \frac{(n-i)^{n-i} (i-1)^{i-1}}{(n-1)^{n-1}}
$$
$$
\bernstein{i}{n}' (u_+) = - { n \choose i } \frac{(i)^i (n-i-1)^{n-i-1}}{(n-1)^{n-1}}
$$

Then

$$ M_{i,n}'(I) = \max(|\bernstein{i}{n}' (t_0)|,|\bernstein{i}{n}' (t_1)|,|\bernstein{i}{n}' (u_+)|,|\bernstein{i}{n}' (u_-)|)$$


\end{document}
